add coins example

src/grw_mon.v
@@ -1,6 +1,8 @@
 Require Import CrossCrypto.fmap.list_of_pairs.
 Require CrossCrypto.fmap.
 Require Import FCF.FCF FCF.EqDec.
+Require Import Coq.Classes.Morphisms.
+Require Import CrossCrypto.RewriteUtil.
 
 Definition mapops V := list_of_pairs (V:=V) (Nat.eqb).
 Notation map V := (mapops V).(fmap.M).
@@ -14,6 +16,10 @@ Inductive type : Type :=
 | tnat : type
 | tbool : type
 | tprod : type -> type -> type.
+
+Bind Scope etype_scope with type.
+Delimit Scope etype_scope with etype.
+Local Notation "A * B" := (tprod A%etype B%etype) : etype_scope.
 
 Fixpoint interp_type (t : type) : Set :=
   match t with
@@ -45,19 +51,34 @@ Definition ftensor {t1 t2 t1' t2'} (f : func t1 t2) (f' : func t1' t2')
   fun '(x, x') => y <-$ f x; y' <-$ f' x'; ret (y, y').
 
 Inductive expr : type -> type -> Type :=
-| ecconst {t1 t2} : cfunc t1 t2 -> expr t1 t2
-| econst {t1 t2} : func t1 t2 -> expr t1 t2
-| ecompose {t1 t2 t3} : expr t1 t2 -> expr t2 t3 -> expr t1 t3
-| etensor {t1 t1' t2 t2'} :
+| cconst {t1 t2} : cfunc t1 t2 -> expr t1 t2
+| const {t1 t2} : func t1 t2 -> expr t1 t2
+| compose {t1 t2 t3} : expr t1 t2 -> expr t2 t3 -> expr t1 t3
+| tensor {t1 t1' t2 t2'} :
     expr t1 t2 -> expr t1' t2' -> expr (tprod t1 t1') (tprod t2 t2').
+
+Bind Scope expr_scope with expr.
+Delimit Scope expr_scope with expr.
+Local Notation "'[[' x ']]'" := (cconst x)
+                            (format "[[ x ]]") : expr_scope.
+Local Notation "'#' x" := (const x)
+                            (no associativity,
+                             at level 9,
+                             format "# x") : expr_scope.
+Local Notation "f1 * f2" := (tensor f1%expr f2%expr)
+                              (left associativity,
+                               at level 40) : expr_scope.
+Local Notation "f @ g" := (compose f%expr g%expr)
+                            (right associativity,
+                             at level 41) : expr_scope.
 
 Fixpoint interp_expr {t1 t2} (e : expr t1 t2) : func t1 t2 :=
   match e with
-  | ecconst cf => liftc cf
-  | econst f => f
-  | ecompose e1 e2 => fcompose (interp_expr e1) (interp_expr e2)
-  | etensor e e' => ftensor (interp_expr e) (interp_expr e')
-  end.
+  | [[cf]] => liftc cf
+  | #f => f
+  | e1 @ e2 => fcompose (interp_expr e1) (interp_expr e2)
+  | e * e' => ftensor (interp_expr e) (interp_expr e')
+  end%expr.
 
 Fixpoint tmap (m : map type) : type :=
   match m with
@@ -65,7 +86,7 @@ Fixpoint tmap (m : map type) : type :=
   | cons (_, t) m => tprod t (tmap m)
   end.
 
-Definition empty : cfunc tunit (tmap mempty) := fun _ => tt.
+(* empty is just id_unit *)
 
 Definition find (m : map type) (i : nat) (l : interp_type (tmap m))
   : match mfind i m with
@@ -83,6 +104,156 @@ Defined.
 Definition add (m : map type) (i : nat) (t : type) (x : interp_type t)
   (l : interp_type (tmap m)) : interp_type (tmap (madd i t m)) := (x, l).
 
-Definition fadd (m : map type) (i : nat) (t : type)
+Definition fadd {m : map type} (i : nat) {t : type}
   : cfunc (tprod t (tmap m)) (tmap (madd i t m)) :=
   fun '(x, l) => add m i t x l.
+
+Definition copy {t} : cfunc t (tprod t t) :=
+  fun x => (x, x).
+Definition delete {t} : cfunc t tunit :=
+  fun _ => tt.
+Definition swap {t1 t2} : cfunc (tprod t1 t2) (tprod t2 t1) :=
+  fun '(t1, t2) => (t2, t1).
+
+Definition units (t : type) :
+  cfunc tunit
+        ((fix units_type t :=
+            match t with
+            | t1 * t2 =>
+              (units_type t1) * (units_type t2)
+            | _ => tunit
+            end%etype) t).
+  induction t; try exact delete.
+  intros ?; cbn [interp_type]; eauto.
+Defined.
+
+Definition fequiv {t1 t2} (f f' : func t1 t2) : Prop :=
+  forall x, Comp_eq (f x) (f' x).
+
+Local Instance Equivalence_fequiv {t1 t2} : Equivalence (@fequiv t1 t2).
+Proof.
+  split; cbv [fequiv Reflexive Symmetric Transitive]; intros;
+    solve [(reflexivity + symmetry + etransitivity); eauto].
+Qed.
+
+Definition cfequiv {t1 t2} (f f' : cfunc t1 t2) : Prop :=
+  forall x, f x = f' x.
+
+Local Instance Equivalence_cfequiv {t1 t2} : Equivalence (@cfequiv t1 t2).
+Proof.
+  split; cbv [cfequiv Reflexive Symmetric Transitive]; intros;
+    solve [(reflexivity + symmetry + etransitivity); eauto].
+Qed.
+
+Lemma cfequiv_fequiv {t1 t2} (f f' : cfunc t1 t2) :
+  cfequiv f f' -> fequiv (liftc f) (liftc f').
+Proof.
+  cbv [cfequiv fequiv liftc].
+  intros H ?; setoid_rewrite H; reflexivity.
+Qed.
+
+Definition equiv {t1 t2} (e e' : expr t1 t2) : Prop :=
+  fequiv (interp_expr e) (interp_expr e').
+
+Local Instance Equivalence_equiv {t1 t2} : Equivalence (@equiv t1 t2).
+Proof.
+  split; cbv [equiv Reflexive Symmetric Transitive]; intros;
+    solve [(reflexivity + symmetry + etransitivity); eauto].
+Qed.
+
+Section ExampleCoins.
+  Definition coin : func tunit tbool :=
+    fun _ => x <-$ Rnd 1; ret (Vector.nth x Fin.F1).
+
+  Definition xor' : cfunc (tprod tbool tbool) tbool :=
+    fun '(x, y) => xorb x y.
+
+  Lemma coins_xor :
+    equiv ([[units (tunit * tunit)]]
+             @ (#coin * #coin)
+             @ [[xor']])
+          #coin.
+  Proof.
+    cbv [equiv fequiv interp_type interp_expr fcompose ftensor liftc coin xor' units type_rect delete].
+    intros _.
+    repeat (setoid_rewrite Bind_Ret_l || setoid_rewrite <-Bind_assoc).
+    cbv [Comp_eq image_relation pointwise_relation evalDist getSupport
+        getAllBvectors].
+    cbn [List.map app sumList fold_left
+                  Vector.nth xorb Vector.caseS
+                  expnat Nat.mul Nat.add].
+    generalize (@EqDec_dec bool (@interp_type_eqdec tbool));
+      intros d0.
+    generalize (EqDec_dec bool_EqDec); intros d1.
+    intros a.
+    destruct (d0 true a), (d0 false a); try congruence;
+      destruct (d1 true a), (d1 false a); try congruence;
+        reflexivity.
+  Qed.
+
+  Fixpoint associate_type (t : type) : type :=
+    match t with
+    | tprod t1 t2 =>
+      match associate_type t1 with
+      | tunit => associate_type t2
+      | t1' => match associate_type t2 with
+               | tunit => t1'
+               | tprod t2a t2b => tprod (tprod t1' t2a) t2b
+               | t2' => tprod t1' t2'
+               end
+      end
+    | _ => t
+    end.
+
+  Fixpoint associate (t : type) : cfunc t (associate_type t).
+    cbv [cfunc].
+    induction t; cbn [associate_type]; eauto.
+    intros [x y].
+    destruct (associate_type t1);
+      [eauto |
+       destruct (associate_type t2);
+       [apply IHt1; eauto |
+        split; [apply IHt1 | apply IHt2]; eauto |
+        split; [apply IHt1 | apply IHt2]; eauto |
+        split; [split|]; [apply IHt1; eauto|..];
+        edestruct IHt2; eauto] ..].
+  Defined.
+
+  Definition unassociate (t : type) : cfunc (associate_type t) t.
+    cbv [cfunc].
+    induction t; cbn [associate_type interp_type]; eauto.
+    intros x.
+    destruct (associate_type t1); cbn [interp_type] in *;
+      [eauto using pair, tt |
+       destruct (associate_type t2); cbn [interp_type] in *;
+       [split; [apply IHt1 | apply IHt2]; eauto using tt |
+        destruct x as [x y]; split; [apply IHt1; exact x |
+                                     apply IHt2; exact y] .. |
+        destruct x as ((x&y)&z); split; [apply IHt1; exact x |
+                                         apply IHt2; exact (y, z)] ] ..].
+  Defined.
+
+  Example coins_example : expr tunit (tbool * (tbool * tbool)) :=
+    ([[units (tunit * tmap nil)]]
+      @ (#coin * [[id]])
+       @ [[fadd 0]]
+       @ [[copy]]
+       @ (([[delete]] @ #coin) * [[id]])
+       @ [[fadd 1]]
+       @ [[copy]]
+       @ (([[delete]] @ #coin) * [[id]])
+       @ [[fadd 2]]
+       @ [[copy]]
+       @ ((([[copy]] @ ([[copy]] * [[id]]))
+             @ (let m := (madd 2 tbool (madd 1%nat tbool (madd 0%nat tbool mempty))) in
+                [[delete]] * [[find m 0]] * [[find m 2]])
+             @ [[associate (tunit * tbool * tbool)]]
+             @ [[xor']])
+          * [[id]])
+       @ [[fadd 3]]
+       @ ([[copy]] @ ([[id]] * ([[copy]] @ ([[id]] * [[copy]]))))
+       @ (let m := (madd 3 tbool (madd 2 tbool (madd 1%nat tbool (madd 0%nat tbool mempty)))) in
+          [[find m 3]] * ([[find m 1]] * ([[find m 1]] * [[delete]])))
+       @ [[associate (tbool * (tbool * (tbool * tunit)))]]
+       @ [[unassociate (tbool * (tbool * tbool))]])%expr.
+End ExampleCoins.
